sha/hmac_NK.v
@@ -2,22 +2,19 @@ Require Import Clightdefs.
 
 Require Import sha.sha.
 Definition t_struct_SHA256state_st := sha.t_struct_SHA256state_st.
-(*
-Definition _o_ctx : ident := 141%positive.
-Definition _ctx_key : ident := 153%positive.
-*)
+
 Local Open Scope Z_scope.
 
-Definition _HMAC : ident := 1165%positive.
+Definition _m__1 : ident := 1165%positive.
 Definition _SHA256_Final : ident := 1140%positive.
 Definition ___compcert_va_int64 : ident := 1116%positive.
 Definition _SHA256_Init : ident := 1138%positive.
 Definition _key : ident := 1146%positive.
-Definition _d : ident := 1162%positive.
-Definition _HMAC_Init : ident := 1154%positive.
+Definition _n : ident := 1162%positive.
+Definition _HMAC_Update : ident := 1154%positive.
 Definition ___builtin_fmax : ident := 1122%positive.
 Definition ___builtin_va_arg : ident := 1112%positive.
-Definition _n : ident := 1163%positive.
+Definition _c : ident := 1163%positive.
 Definition ___builtin_annot_intval : ident := 1110%positive.
 Definition _struct_hmac_ctx_st : ident := 1144%positive.
 Definition ___builtin_negl : ident := 113%positive.
@@ -25,11 +22,10 @@ Definition ___builtin_write32_reversed : ident := 112%positive.
 Definition ___builtin_write16_reversed : ident := 111%positive.
 Definition _memset : ident := 1131%positive.
 Definition _j : ident := 1149%positive.
-Definition _m__1 : ident := 1166%positive.
-Definition _HMAC_cleanup : ident := 1159%positive.
+Definition _HMAC2 : ident := 1166%positive.
+Definition _m : ident := 1159%positive.
 Definition ___builtin_addl : ident := 114%positive.
-Definition _main : ident := 1168%positive.
-Definition _HMAC_Final : ident := 1158%positive.
+Definition _HMAC_cleanup : ident := 1158%positive.
 Definition ___builtin_read16_reversed : ident := 1128%positive.
 Definition ___builtin_fabs : ident := 117%positive.
 Definition ___builtin_fsqrt : ident := 1121%positive.
@@ -38,39 +34,39 @@ Definition _ctx : ident := 1145%positive.
 Definition ___builtin_va_copy : ident := 1113%positive.
 Definition ___builtin_fnmsub : ident := 1127%positive.
 Definition _data : ident := 1133%positive.
-Definition _md : ident := 1156%positive.
+Definition _buf : ident := 1156%positive.
 Definition ___builtin_fmsub : ident := 1125%positive.
 Definition ___compcert_va_int32 : ident := 1115%positive.
-Definition _m : ident := 1160%positive.
+Definition _key_len : ident := 1160%positive.
 Definition ___builtin_bswap16 : ident := 1120%positive.
 Definition _num : ident := 1132%positive.
 Definition ___builtin_fmadd : ident := 1124%positive.
-Definition _HMAC2 : ident := 1167%positive.
+Definition _main : ident := 1167%positive.
 Definition ___compcert_va_float64 : ident := 1117%positive.
 Definition ___builtin_memcpy_aligned : ident := 118%positive.
 Definition ___builtin_subl : ident := 115%positive.
 Definition _reset : ident := 1150%positive.
 Definition _md_ctx : ident := 1143%positive.
-Definition _ctx_key : ident := 1153%positive.
+Definition _HMAC_Init : ident := 1153%positive.
 Definition _len : ident := 1147%positive.
-Definition _buf : ident := 1157%positive.
+Definition _HMAC_Final : ident := 1157%positive.
 Definition _h : ident := 1136%positive.
 Definition ___builtin_va_end : ident := 1114%positive.
 Definition ___builtin_mull : ident := 116%positive.
 Definition ___builtin_fnmadd : ident := 1126%positive.
 Definition ___builtin_bswap32 : ident := 1119%positive.
 Definition _SHA256_Update : ident := 1139%positive.
-Definition _key_len : ident := 1161%positive.
+Definition _d : ident := 1161%positive.
 Definition ___builtin_va_start : ident := 1111%positive.
 Definition _struct_SHA256state_st : ident := 1137%positive.
 Definition _i_ctx : ident := 1142%positive.
 Definition ___builtin_annot : ident := 119%positive.
-Definition _c : ident := 1164%positive.
-Definition _ctx_key_length : ident := 1152%positive.
+Definition _HMAC : ident := 1164%positive.
+Definition _ctx_key : ident := 1152%positive.
 Definition _o_ctx : ident := 1141%positive.
 Definition _Nh : ident := 1134%positive.
 Definition ___builtin_read32_reversed : ident := 1129%positive.
-Definition _HMAC_Update : ident := 1155%positive.
+Definition _md : ident := 1155%positive.
 Definition _Nl : ident := 1135%positive.
 Definition _memcpy : ident := 1130%positive.
 Definition ___builtin_fmin : ident := 1123%positive.
@@ -116,8 +112,7 @@ Definition f_HMAC_Init := {|
                 (_key, (tptr tuchar)) :: (_len, tint) :: nil);
   fn_vars := ((_pad, (tarray tuchar 64)) :: (_ctx_key, (tarray tuchar 64)) ::
               nil);
-  fn_temps := ((_i, tint) :: (_j, tint) :: (_reset, tint) ::
-               (_ctx_key_length, tuint) :: nil);
+  fn_temps := ((_i, tint) :: (_j, tint) :: (_reset, tint) :: nil);
   fn_body :=
 (Ssequence
   (Sset _reset (Econst_int (Int.repr 0) tint))
@@ -170,20 +165,18 @@ Definition f_HMAC_Init := {|
                            t_struct_hmac_ctx_st) _md_ctx
                          t_struct_SHA256state_st)
                        (tptr t_struct_SHA256state_st)) :: nil))
-                  (Ssequence
-                    (Scall None
-                      (Evar _memset (Tfunction
-                                      (Tcons (tptr tvoid)
-                                        (Tcons tint (Tcons tuint Tnil)))
-                                      (tptr tvoid) cc_default))
-                      ((Eaddrof
-                         (Ederef
-                           (Ebinop Oadd (Evar _ctx_key (tarray tuchar 64))
-                             (Econst_int (Int.repr 32) tint) (tptr tuchar))
-                           tuchar) (tptr tuchar)) ::
-                       (Econst_int (Int.repr 0) tint) ::
-                       (Econst_int (Int.repr 32) tint) :: nil))
-                    (Sset _ctx_key_length (Econst_int (Int.repr 32) tint))))))
+                  (Scall None
+                    (Evar _memset (Tfunction
+                                    (Tcons (tptr tvoid)
+                                      (Tcons tint (Tcons tuint Tnil)))
+                                    (tptr tvoid) cc_default))
+                    ((Eaddrof
+                       (Ederef
+                         (Ebinop Oadd (Evar _ctx_key (tarray tuchar 64))
+                           (Econst_int (Int.repr 32) tint) (tptr tuchar))
+                         tuchar) (tptr tuchar)) ::
+                     (Econst_int (Int.repr 0) tint) ::
+                     (Econst_int (Int.repr 32) tint) :: nil)))))
             (Ssequence
               (Scall None
                 (Evar _memcpy (Tfunction
@@ -193,20 +186,18 @@ Definition f_HMAC_Init := {|
                 ((Evar _ctx_key (tarray tuchar 64)) ::
                  (Etempvar _key (tptr tuchar)) :: (Etempvar _len tint) ::
                  nil))
-              (Ssequence
-                (Scall None
-                  (Evar _memset (Tfunction
-                                  (Tcons (tptr tvoid)
-                                    (Tcons tint (Tcons tuint Tnil)))
-                                  (tptr tvoid) cc_default))
-                  ((Eaddrof
-                     (Ederef
-                       (Ebinop Oadd (Evar _ctx_key (tarray tuchar 64))
-                         (Etempvar _len tint) (tptr tuchar)) tuchar)
-                     (tptr tuchar)) :: (Econst_int (Int.repr 0) tint) ::
-                   (Ebinop Osub (Econst_int (Int.repr 64) tuint)
-                     (Etempvar _len tint) tuint) :: nil))
-                (Sset _ctx_key_length (Etempvar _len tint)))))))
+              (Scall None
+                (Evar _memset (Tfunction
+                                (Tcons (tptr tvoid)
+                                  (Tcons tint (Tcons tuint Tnil)))
+                                (tptr tvoid) cc_default))
+                ((Eaddrof
+                   (Ederef
+                     (Ebinop Oadd (Evar _ctx_key (tarray tuchar 64))
+                       (Etempvar _len tint) (tptr tuchar)) tuchar)
+                   (tptr tuchar)) :: (Econst_int (Int.repr 0) tint) ::
+                 (Ebinop Osub (Econst_int (Int.repr 64) tuint)
+                   (Etempvar _len tint) tuint) :: nil))))))
       Sskip)
     (Ssequence
       (Sifthenelse (Etempvar _reset tint)
